wip

pulse/examples/steel/DList.Invariant.fst
@@ -51,182 +51,393 @@ let ptr_eq (#a:Type) (x y:t a) = admit()
 ////////////////////////////////////////////////////////////////////////////////
 // Main dlist invariant
 ////////////////////////////////////////////////////////////////////////////////
-let rec dlist' (#a:Type) (left:t a)
-                        (ptr:t a)
-                        (right:t a)
-                        (l:list (cell a))
-    : Tot slprop (decreases l)
-    =
-    match l with
-    | [] ->
-      pure (right == ptr)
+(**
+ *
+ *  dlist left ptr tail right [d0;...;dn]
+ *
+ *  left    ptr               tail       right
+ *  |        |                  |         |
+ *  |        v                  v         |
+ *  v       __         __       __        v
+ *  <-prev-|d0|-next->|  | ... |dn|-next->
+ *         |__|<-prev-|__| ..  |__|
+ *
+ *
+ * dlist left ptr tail right []
+ *   ptr
+ *)
 
-    | hd :: tl ->
-      pure (right =!= ptr) `star`
-      pts_to ptr full_perm hd `star`
-      pure (prev hd == left) `star`
-      dlist' ptr (next hd) right tl
-let dlist = dlist'
+let repr (a:Type) = l:list (cell a) { Cons? l }
+
+let rec dlist_cons (#a:Type) (previous :t a)
+                             (cur  :t a)
+                             (last :t a)
+                             (right:t a)
+                             (xs:repr a)
+    : Tot slprop (decreases xs)
+    = match xs with
+      | [ x ]  ->
+        pure (cur == last /\
+              prev x == previous /\
+              next x == right) `star`
+        pts_to cur full_perm x
+
+      | x :: xs' ->
+        pure (prev x == previous) `star`
+        pts_to cur full_perm x `star`
+        dlist_cons cur (next x) last right xs'
+
+let rec dlist_snoc (#a:Type) (left:t a)
+                             (last:t a)
+                             (cur:t a)
+                             (nxt:t a)
+                             (xs:repr a)
+    : Tot slprop (decreases xs)
+    = match xs with
+      | [ x ]  ->
+        pure (cur == last /\
+              prev x == left /\
+              next x == nxt) `star`
+        pts_to cur full_perm x
+
+      | x :: xs' ->
+        pure (next x == nxt) `star`
+        pts_to cur full_perm x `star`
+        dlist_snoc left last (prev x) cur xs'
+
+let dlist_cons_snoc_nil #a (left front back right: t a) (x:_)
+  : Lemma (dlist_cons left front back right [x] `equiv`
+           dlist_snoc left front back right [x])
+  = calc (equiv) {
+         dlist_cons left front back right [x];
+      (equiv) {}
+         pure (front == back /\
+               prev x == left /\
+               next x == right) `star`
+         pts_to front full_perm x;
+       (equiv) { assume (front == back) }
+         pure (front == back /\
+               prev x == left /\
+               next x == right) `star`
+         pts_to back full_perm x;
+       (equiv) { admit () }
+         pure (back == front /\
+               prev x == left /\
+               next x == right) `star`
+         pts_to back full_perm x;
+    }
+
+module ST = Steel.Memory.Tactics
+let dlist_snoc_snoc_1 (#a:Type) (left:t a)
+                                 (last:t a)
+                                 (cur:t a)
+                                 (right:t a)
+                                 (x0:cell a)
+                                 (x:cell a)
+  : Lemma (ensures
+          (dlist_snoc left last cur right [x0;x] `equiv`
+            (pure (prev x == left) `star`
+             pts_to last full_perm x `star`
+             dlist_snoc last (next x) cur right [x0])))
+  = calc (equiv) {
+         dlist_snoc left last cur right [x0;x];
+    (equiv) { }
+         pure (next x0 == right) `star`
+         pts_to cur full_perm x0 `star`
+         dlist_snoc left last (prev x0) cur [x];
+    (equiv) { }
+         pure (next x0 == right) `star`
+         pts_to cur full_perm x0 `star`
+         (pure (prev x0 == last /\
+                prev x == left /\
+                next x == cur) `star`
+          pts_to (prev x0) full_perm x);
+    (equiv) { admit() }
+         pure (prev x == left) `star`
+         pts_to last full_perm x `star`
+         (pure (cur == next x /\
+                prev x0 == last /\
+                next x0 == right) `star`
+          pts_to cur full_perm x0)                ;
+    }
+
+assume
+val equiv_extensional_on_star_r (p1 p2 p3:slprop)
+  : squash (p2 `equiv` p3 ==> (p1 `star` p2) `equiv` (p1 `star` p3))
+
+assume
+val gather_pure (p q:prop) : Lemma ((pure p `star` pure q) == pure (p /\ q))
+assume
+val rewrite_pure (p q:prop) : Lemma (requires (p <==> q)) (ensures (pure p `equiv` pure q))
+
+#push-options "--z3rlimit_factor 4"
+assume
+val utils (_:unit)
+  : Lemma ((forall p q r. ((p `star` q) `star` r) == (p `star` (q `star` r))) /\
+           (forall p q. (p `star` q) == (q `star` p)) /\
+           (forall p q.{:pattern (p `equiv` q)} (p `equiv` q) <==> p == q) /\
+           (forall (a b:prop).{:pattern (pure a);(pure b)} (a <==> b) <==> (pure a == pure b)) /\
+           (forall (a b:prop). {:pattern (pure a `star` pure b)} ((pure a) `star` (pure b)) `equiv` pure (a /\ b)))
+#pop-options
+#push-options "--query_stats --initial_fuel 2 --initial_ifuel 1 --max_fuel 2 --max_ifuel 1 --z3rlimit_factor 4"
+module T = FStar.Tactics
+
+let no_prev_cycles #a (left last cur right: _) (p:_) (v:_) (xs:repr a) (m:_)
+  : Lemma (requires (interp (pts_to p full_perm v `star` dlist_snoc left last cur right xs) m))
+          (ensures (forall c. List.memP c xs ==> prev c =!= p) /\ p =!= last /\ p =!= cur)
+  = admit()
+
+let no_next_cycles #a (left cur last right: _) (p:_) (v:_) (xs:repr a) (m:_)
+  : Lemma (requires interp (pts_to p full_perm v `star` dlist_cons left cur last right xs) m)
+          (ensures (forall c. List.memP c xs ==> next c =!= p) /\ p =!= last /\ p =!= cur)
+  = admit()
+
+let stronger (p q:slprop) = forall m. interp p m ==> interp q m
+let stronger_drop (#p #q #r:slprop) : Lemma ((p `star` q) `stronger` q) = ()
+let stronger_equiv (#p #q #r:slprop) : Lemma ((p `equiv` q) ==> p `stronger` q) = ()
 
 
-// assume
-// val dlist_injective (#a:_) (left ptr right : t a)
-//                            (l1 l2:list (cell a))
-//                            (h:mem)
-//   : Lemma
-//     (requires
-//       interp (dlist left ptr right l1) h /\
-//       interp (dlist left ptr right l2) h)
-//     (ensures
-//       l1 == l2)
-//    (decreases l1)
-//   = match l1, l2 with
-//     | [], [] -> ()
-//     | hd1::tl1, hd2::tl2 ->
-//       pts_to_injective ptr hd1 hd2 h;
-//       assert (hd1 == hd2);
-//       dlist_injective' ptr hd1.next right tl1 tl2 h
+let rec dlist_snoc_snoc (#a:Type) (left:t a)
+                                  (last:t a)
+                                  (cur:t a)
+                                  (right:t a)
+                                  (xs:repr a)
+                                  (x:cell a)
+  : Lemma (ensures
+          (dlist_snoc left last cur right (List.snoc (xs, x)) `equiv`
+            (pure (prev x == left) `star`
+             pts_to last full_perm x `star`
+             dlist_snoc last (next x) cur right xs)))
+          (decreases (List.length xs))
+  = match xs with
+    | [hd] -> dlist_snoc_snoc_1 left last cur right hd x
+    | hd::xs' ->
+      let xs' : repr a = xs' in
+      calc (equiv) {
+        dlist_snoc left last cur right (List.snoc (hd::xs', x));
+      (equiv) { (* defn *) }
+        pure (next hd == right) `star`
+        pts_to cur full_perm hd `star`
+        dlist_snoc left last (prev hd) cur (List.snoc (xs', x));
+      (equiv) { (* IH *)
+                utils ();
+                dlist_snoc_snoc left last (prev hd) cur xs' x
+              }
+        pure (next hd == right) `star`
+        pts_to cur full_perm hd `star`
+        (pure (prev x == left) `star`
+         pts_to last full_perm x `star`
+         dlist_snoc last (next x) (prev hd) cur xs');
+      (equiv) { (* boring *) _ by (ST.canon()) }
+        pure (prev x == left) `star`
+        pts_to last full_perm x `star`
+        (pure (next hd == right) `star`
+         pts_to cur full_perm hd `star`
+         dlist_snoc last (next x) (prev hd) cur xs');
+      (equiv) { }
+         (pure (prev x == left) `star`
+          pts_to last full_perm x `star`
+          dlist_snoc last (next x) cur right xs);
+      }
 
-//     | [], hd::tl
-//     | hd::tl, [] ->
-//       elim_pure (right == ptr) h;
-//       elim_pure (right =!= ptr) h
-// let dlist_injective = dlist_injective'
-
-#push-options "--query_stats --fuel 1,1 --ifuel 1,1"
-let intro_dlist_nil (#a:Type) (left right:t a)
-   : SteelT unit emp (fun _ -> dlist left right right [])
-   = change_slprop emp (dlist left right right [])
-                       (fun m -> pure_interp (right == right) m;
-                              norm_spec [delta;zeta] ((dlist left right right [])))
-
-let elim_dlist_nil (#a:Type) (left ptr right:t a)
-   : SteelT unit
-     (dlist left ptr right [])
-     (fun _ -> pure (right == ptr))
-   = change_slprop (dlist left ptr right [])
-                   (pure (right == ptr))
-                   (fun m -> pure_interp (ptr == right) m;
-                          norm_spec [delta;zeta] ((dlist left ptr right [])))
+let rev #a (r:repr a) : repr a = let x = List.rev r in assume (Cons? x); x
 
 
-let intro_star_pure (p:slprop) (q:prop) (h:mem)
-  : Lemma (interp p h /\ q ==> interp (p `star` pure q) h)
-  = let open Steel.Memory in
-    emp_unit p;
-    pure_star_interp p q h
-
-let dlist_right_right_nil (#a:Type) (left right:t a) (l:list (cell a)) (m:mem)
-  : Lemma
-    (requires interp (dlist left right right l) m)
-    (ensures interp (dlist left right right [] `star` pure (l == [])) m)
-  = pure_interp (right == right) m;
-    pure_interp (right =!= right) m;
-    pure_interp (l == []) m;
-    match l with
-    | [] -> intro_star_pure (dlist left right right []) (l == []) m
-    | hd::tl -> norm_spec [delta;zeta] (dlist left right right (hd::tl))
-
-let invert_dlist_nil_eq (#a:Type) (left ptr right:t a) (l:list (cell a))
-    : Steel unit
-            (dlist left ptr right l)
-            (fun _ -> dlist left right right [] `star` pure (l==[]))
-            (requires fun _ -> ptr == right)
-            (ensures fun _ _ _ -> True)
-    = change_slprop (dlist left ptr right l)
-                    (dlist left right right l)
-                    (fun _ -> ());
-      change_slprop (dlist left right right l)
-                    (dlist left right right [] `star` pure (l == []))
-                    (dlist_right_right_nil left right l)
-
-let intro_dlist_cons (#a:Type) (left:t a)
-                               (ptr:t a)
-                               (right:t a)
-                               (hd: cell a)
-                               (tl: list (cell a))
-   : Steel unit
-     (pts_to ptr full_perm hd `star` dlist ptr (next hd) right tl)
-     (fun _ -> dlist left ptr right (hd::tl))
-     (requires fun _ ->
-       prev hd == left /\
-       ptr =!= right)
-     (ensures fun _ _ _ -> True)
-   = change_slprop emp (pure (prev hd == left)) (fun m -> pure_interp (prev hd == left) m);
-     change_slprop emp (pure (right =!= ptr)) (fun m -> pure_interp (right =!= ptr) m);
-     change_slprop  (pure (right =!= ptr) `star`
-                     pts_to ptr full_perm hd `star`
-                     pure (prev hd == left) `star`
-                     dlist ptr (next hd) right tl)
-                    (dlist left ptr right (hd::tl))
-                    (fun _ -> norm_spec [delta;zeta] (dlist left ptr right (hd::tl)))
-
-let elim_dlist_cons (#a:Type) (left:t a)
-                              (ptr:t a)
-                              (right:t a)
-                              (hd:cell a)
-                              (tl:list (cell a))
-   = change_slprop  (dlist left ptr right (hd::tl))
-                    (pure (right =!= ptr) `star`
-                     pts_to ptr full_perm hd `star`
-                     pure (prev hd == left) `star`
-                     dlist ptr (next hd) right tl)
-                    (fun _ -> norm_spec [delta;zeta] (dlist left ptr right (hd::tl)));
-     U.elim_pure (right =!= ptr);
-     U.elim_pure (prev hd == left)
-
-let lemma_invert_dlist_cons_neq (#a:Type) (left ptr right:t a) (l:list (cell a)) (m:mem)
-  : Lemma
-    (requires interp (dlist left ptr right l) m /\ ptr =!= right)
-    (ensures interp (dlist left ptr right l `star` pure (Cons? l == true)) m)
+let rec dlist_cons_snoc (#a:Type) (left :t a)
+                                  (head  :t a)
+                                  (tail :t a)
+                                  (right:t a)
+                                  (l:repr a)
+  : Lemma (ensures dlist_cons left head tail right l `equiv`
+                   dlist_snoc left head tail right (rev l))
+          (decreases l)
   = match l with
-    | [] ->
-      norm_spec [delta;zeta] (dlist left ptr right []);
-      assert (interp (dlist left ptr right []) m);
-      pure_interp (right == ptr) m
-    | hd::tl ->
-      intro_star_pure (dlist left ptr right l) (Cons? l == true) m
+    | [x] -> dlist_cons_snoc_nil left head tail right x
+    | x :: xs ->
+      dlist_cons_snoc head (next x) tail right xs;
+      assert (dlist_cons head (next x) tail right xs `equiv`
+              dlist_snoc head (next x) tail right (rev xs));
+      assume (rev l == List.snoc (rev xs, x));
+      calc (equiv) {
+        dlist_cons left head tail right (x::xs);
+      (equiv) { }
+          pure (prev x == left)
+          `star`
+          pts_to head full_perm x `star`
+          dlist_cons head (next x) tail right xs;
+       (equiv) { equiv_extensional_on_star_r
+                         (pure (prev x == left)
+                               `star`
+                          pts_to head full_perm x)
+                          (dlist_cons head (next x) tail right xs)
+                          (dlist_snoc head (next x) tail right (rev xs))
+                }
+          pure (prev x == left)
+          `star`
+          pts_to head full_perm x `star`
+          (dlist_snoc head (next x) tail right (rev xs));
+      };
+      dlist_snoc_snoc left head tail right (rev xs) x
 
-let invert_dlist_cons_neq (#a:Type) (left ptr right:t a) (l:list (cell a))
-    : Steel unit
-     (requires
-       dlist left ptr right l)
-     (ensures fun _ ->
-       dlist left ptr right l)
-     (requires fun _ ->
-       ptr =!= right)
-     (ensures fun _ _ _ ->
-       Cons? l == true)
-   = change_slprop (dlist left ptr right l)
-                   (dlist left ptr right l `star` pure (Cons? l == true))
-                   (lemma_invert_dlist_cons_neq left ptr right l);
-     U.elim_pure (Cons? l == true)
+
+// // assume
+// // val dlist_injective (#a:_) (left ptr right : t a)
+// //                            (l1 l2:list (cell a))
+// //                            (h:mem)
+// //   : Lemma
+// //     (requires
+// //       interp (dlist left ptr right l1) h /\
+// //       interp (dlist left ptr right l2) h)
+// //     (ensures
+// //       l1 == l2)
+// //    (decreases l1)
+// //   = match l1, l2 with
+// //     | [], [] -> ()
+// //     | hd1::tl1, hd2::tl2 ->
+// //       pts_to_injective ptr hd1 hd2 h;
+// //       assert (hd1 == hd2);
+// //       dlist_injective' ptr hd1.next right tl1 tl2 h
+
+// //     | [], hd::tl
+// //     | hd::tl, [] ->
+// //       elim_pure (right == ptr) h;
+// //       elim_pure (right =!= ptr) h
+// // let dlist_injective = dlist_injective'
+
+// #push-options "--query_stats --fuel 1,1 --ifuel 1,1"
+// let intro_dlist_nil (#a:Type) (left right:t a)
+//    : SteelT unit emp (fun _ -> dlist left right right [])
+//    = change_slprop emp (dlist left right right [])
+//                        (fun m -> pure_interp (right == right) m;
+//                               norm_spec [delta;zeta] ((dlist left right right [])))
+
+// let elim_dlist_nil (#a:Type) (left ptr right:t a)
+//    : SteelT unit
+//      (dlist left ptr right [])
+//      (fun _ -> pure (right == ptr))
+//    = change_slprop (dlist left ptr right [])
+//                    (pure (right == ptr))
+//                    (fun m -> pure_interp (ptr == right) m;
+//                           norm_spec [delta;zeta] ((dlist left ptr right [])))
 
 
-////////////////////////////////////////////////////////////////////////////////
+// let intro_star_pure (p:slprop) (q:prop) (h:mem)
+//   : Lemma (interp p h /\ q ==> interp (p `star` pure q) h)
+//   = let open Steel.Memory in
+//     emp_unit p;
+//     pure_star_interp p q h
 
-let dlist_not_null (#a:Type)
-                   (#left:t a)
-                   (#right:t a)
-                   (#rep:list (cell a))
-                   (p:t a)
-  = U.lift_lemma (dlist left p right rep)
-                 ((Cons? rep) == true)
-                 (fun m -> if Cons? rep
-                        then ()
-                        else (assert (p =!= right);
-                              lemma_invert_dlist_cons_neq left p right rep m);
-                              Steel.Memory.pure_star_interp
-                                (dlist left p right rep)
-                                (Cons? rep == true)
-                                m);
-    let hd :: tl = rep in
-    change_slprop (dlist left p right rep)
-                  (dlist left p right (hd :: tl))
-                  (fun _ -> ());
-    elim_dlist_cons left p right hd tl;
-    U.pts_to_not_null #_ #_ #full_perm #(Ghost.hide hd) p;
-    intro_dlist_cons left p right hd tl;
-    change_slprop (dlist left p right (hd :: tl))
-                  (dlist left p right rep)
-                  (fun _ -> ())
+// let dlist_right_right_nil (#a:Type) (left right:t a) (l:list (cell a)) (m:mem)
+//   : Lemma
+//     (requires interp (dlist left right right l) m)
+//     (ensures interp (dlist left right right [] `star` pure (l == [])) m)
+//   = pure_interp (right == right) m;
+//     pure_interp (right =!= right) m;
+//     pure_interp (l == []) m;
+//     match l with
+//     | [] -> intro_star_pure (dlist left right right []) (l == []) m
+//     | hd::tl -> norm_spec [delta;zeta] (dlist left right right (hd::tl))
+
+// let invert_dlist_nil_eq (#a:Type) (left ptr right:t a) (l:list (cell a))
+//     : Steel unit
+//             (dlist left ptr right l)
+//             (fun _ -> dlist left right right [] `star` pure (l==[]))
+//             (requires fun _ -> ptr == right)
+//             (ensures fun _ _ _ -> True)
+//     = change_slprop (dlist left ptr right l)
+//                     (dlist left right right l)
+//                     (fun _ -> ());
+//       change_slprop (dlist left right right l)
+//                     (dlist left right right [] `star` pure (l == []))
+//                     (dlist_right_right_nil left right l)
+
+// let intro_dlist_cons (#a:Type) (left:t a)
+//                                (ptr:t a)
+//                                (right:t a)
+//                                (hd: cell a)
+//                                (tl: list (cell a))
+//    : Steel unit
+//      (pts_to ptr full_perm hd `star` dlist ptr (next hd) right tl)
+//      (fun _ -> dlist left ptr right (hd::tl))
+//      (requires fun _ ->
+//        prev hd == left /\
+//        ptr =!= right)
+//      (ensures fun _ _ _ -> True)
+//    = change_slprop emp (pure (prev hd == left)) (fun m -> pure_interp (prev hd == left) m);
+//      change_slprop emp (pure (right =!= ptr)) (fun m -> pure_interp (right =!= ptr) m);
+//      change_slprop  (pure (right =!= ptr) `star`
+//                      pts_to ptr full_perm hd `star`
+//                      pure (prev hd == left) `star`
+//                      dlist ptr (next hd) right tl)
+//                     (dlist left ptr right (hd::tl))
+//                     (fun _ -> norm_spec [delta;zeta] (dlist left ptr right (hd::tl)))
+
+// let elim_dlist_cons (#a:Type) (left:t a)
+//                               (ptr:t a)
+//                               (right:t a)
+//                               (hd:cell a)
+//                               (tl:list (cell a))
+//    = change_slprop  (dlist left ptr right (hd::tl))
+//                     (pure (right =!= ptr) `star`
+//                      pts_to ptr full_perm hd `star`
+//                      pure (prev hd == left) `star`
+//                      dlist ptr (next hd) right tl)
+//                     (fun _ -> norm_spec [delta;zeta] (dlist left ptr right (hd::tl)));
+//      U.elim_pure (right =!= ptr);
+//      U.elim_pure (prev hd == left)
+
+// let lemma_invert_dlist_cons_neq (#a:Type) (left ptr right:t a) (l:list (cell a)) (m:mem)
+//   : Lemma
+//     (requires interp (dlist left ptr right l) m /\ ptr =!= right)
+//     (ensures interp (dlist left ptr right l `star` pure (Cons? l == true)) m)
+//   = match l with
+//     | [] ->
+//       norm_spec [delta;zeta] (dlist left ptr right []);
+//       assert (interp (dlist left ptr right []) m);
+//       pure_interp (right == ptr) m
+//     | hd::tl ->
+//       intro_star_pure (dlist left ptr right l) (Cons? l == true) m
+
+// let invert_dlist_cons_neq (#a:Type) (left ptr right:t a) (l:list (cell a))
+//     : Steel unit
+//      (requires
+//        dlist left ptr right l)
+//      (ensures fun _ ->
+//        dlist left ptr right l)
+//      (requires fun _ ->
+//        ptr =!= right)
+//      (ensures fun _ _ _ ->
+//        Cons? l == true)
+//    = change_slprop (dlist left ptr right l)
+//                    (dlist left ptr right l `star` pure (Cons? l == true))
+//                    (lemma_invert_dlist_cons_neq left ptr right l);
+//      U.elim_pure (Cons? l == true)
+
+
+// ////////////////////////////////////////////////////////////////////////////////
+
+// let dlist_not_null (#a:Type)
+//                    (#left:t a)
+//                    (#right:t a)
+//                    (#rep:list (cell a))
+//                    (p:t a)
+//   = U.lift_lemma (dlist left p right rep)
+//                  ((Cons? rep) == true)
+//                  (fun m -> if Cons? rep
+//                         then ()
+//                         else (assert (p =!= right);
+//                               lemma_invert_dlist_cons_neq left p right rep m);
+//                               Steel.Memory.pure_star_interp
+//                                 (dlist left p right rep)
+//                                 (Cons? rep == true)
+//                                 m);
+//     let hd :: tl = rep in
+//     change_slprop (dlist left p right rep)
+//                   (dlist left p right (hd :: tl))
+//                   (fun _ -> ());
+//     elim_dlist_cons left p right hd tl;
+//     U.pts_to_not_null #_ #_ #full_perm #(Ghost.hide hd) p;
+//     intro_dlist_cons left p right hd tl;
+//     change_slprop (dlist left p right (hd :: tl))
+//                   (dlist left p right rep)
+//                   (fun _ -> ())
